LLG2FlatImp and test case for it

src/PipelineDemoStepwise.v
@@ -6,6 +6,9 @@ Require Import compiler.Op.
 Require Import compiler.member.
 Require Import compiler.ForWord.
 Require Import compiler.LLG.
+Require compiler.LLG2FlatImp.
+Require Import compiler.FlatImp.
+Require Import compiler.ResMonad.
 
 Definition myvar := nat.
 Definition var_x1: myvar := 3.
@@ -48,4 +51,36 @@ Goal forall n, p1_LLG n = interp_expr' (p1_LLG_ast n). intros. reflexivity. Qed.
 Goal forall n, p1_LLG n = interp_expr' (p1_LLG_ast n).
   intros. unfold p1_LLG. unfold interp_expr', interp_expr. cbn. reflexivity.
 Qed.
+
+Definition nameGenState_initial: myvar := 10. (* should be bigger than all vars used in source *)
+
+Definition compileLLG2FlatImp{l G t}(e: expr l G t): @stmt w myvar * myvar :=
+  fst (LLG2FlatImp.compile nameGenState_initial e).
+
+Definition p1_FlatImp(n: word w): @stmt w myvar * myvar := compileLLG2FlatImp (p1_LLG_ast n).
+
+Definition p1_FlatImp'(n: word w): @stmt w myvar * myvar :=
+  ltac:(let r := eval cbv -[natToWord] in (p1_FlatImp n) in exact r).
+
+Definition p1_FlatImp_stmt(n: word w): @stmt w myvar := 
+  ltac:(let r := eval cbv -[natToWord] in (fst (p1_FlatImp n)) in exact r).
+
+Definition p1_FlatImp_resVar(n: word w): myvar := 
+  ltac:(let r := eval cbv -[natToWord] in (snd (p1_FlatImp n)) in exact r).
+
+Definition lotsOfFuel := 100.
+
+Definition mystate := myvar -> option (word w).
+
+Definition empty_state: mystate := fun _ => None.
+
+Definition eval_FlatImp_stmt(s: @stmt w myvar * myvar): option (word w) :=
+  match eval_stmt lotsOfFuel empty_state (fst s) with
+  | Success final => final (snd s)
+  | _ => None
+  end.
+
+Transparent wlt_dec.
+
+Goal eval_FlatImp_stmt (p1_FlatImp $4) = Some $14. reflexivity. Qed.
 
