src/LLG2FlatImp.v
@@ -1,0 +1,341 @@
+Require Import lib.LibTactics.
+Require Import compiler.Common.
+Require Import compiler.ResMonad.
+Require Import compiler.LLG.
+Require Import compiler.FlatImp.
+Require Import compiler.StateCalculus.
+Require Import compiler.NameGen.
+Require Import compiler.member.
+Require Import compiler.Op.
+
+Section LLG2FlatImp.
+
+  Context {w: nat}. (* bit width *)
+  Context {var: Set}.
+  Context {eq_var_dec: DecidableEq var}.
+  Context {state: Type}.
+  Context {stateMap: Map state var (word w)}.
+  Context {vars: Type}.
+  Context {varset: set vars var}.
+  Context {NGstate: Type}.
+  Context {NG: NameGen var vars NGstate}.
+
+  Definition TODO{T: Type}: T. Admitted.
+
+  Ltac admit_if_TODO :=
+    match goal with
+    | _: context [ TODO ] |- _ => exact TODO
+    | _ => idtac
+    end.
+
+  (* returns and var into which result is saved, and new fresh name generator state
+     TODO use state monad? *)
+  Fixpoint compile{l G t}(ngs: NGstate)(e: @expr w var l G t){struct e}:
+    (@stmt w var * var * NGstate) :=
+    match e with
+    | ELit n => let '(x, ngs') := genFresh ngs in
+                    (SLit x n, x, ngs')
+    | EVar x =>
+        (* (SSkip, x, ngs)  would be simpler but doesn't satisfy the invariant that
+            the returned var is in modVars of the returned statement *)
+        let '(y, ngs') := genFresh ngs in
+        (SSet y (member_get x), y, ngs')
+    | EOp e1 op e2 =>
+        let '(s1, r1, ngs') := compile ngs e1 in
+        let '(s2, r2, ngs'') := compile ngs' e2 in
+        let '(x, ngs''') := genFresh ngs'' in
+        (SSeq s1 (SSeq s2 (SOp x op r1 r2)), x, ngs''')
+    | ELet x e1 e2 =>
+        let '(s1, r1, ngs') := compile ngs e1 in
+        let '(s2, r2, ngs'') := compile ngs' e2 in
+        (SSeq s1 (SSeq (SSet x r1) s2), r2, ngs'')
+    | ENewArray t es => TODO
+    | EGet ea ei => TODO
+    | EUpdate ea ei ev => TODO
+    | EFor i eto upd ebody erest =>
+        let '(to_stmt, to_res, ngs') := compile ngs eto in
+        let '(c, ngs'') := genFresh ngs' in
+        let '(body_stmt, body_res, ngs''') := compile ngs'' ebody in
+        let '(rest_stmt, rest_res, ngs'''') := compile ngs''' erest in
+        let '(one, ngs''''') := genFresh ngs'''' in
+        (SSeq (SLit one $1)
+        (SSeq to_stmt
+        (SSeq (SLit i $0)
+        (SSeq (SLoop (SOp c OLt i to_res)
+                     c
+                     (SSeq body_stmt
+                     (SSeq (SSet (member_get upd) body_res)
+                           (SOp i OPlus i one))))
+         rest_stmt))),
+         rest_res, ngs''''')
+    end.
+
+  Ltac state_calc_instantiation := state_calc var (word w).
+  Ltac state_calc := state_calc_instantiation.
+
+  Lemma compile_freshVarUsage: forall l G t (e: expr l G t) ngs ngs' s v,
+    compile ngs e = (s, v, ngs') ->
+    subset (allFreshVars ngs') (allFreshVars ngs).
+  Proof.
+    induction e; intros; repeat (inversionss; try destruct_one_match_hyp);
+    admit_if_TODO;
+    repeat match goal with
+    | H: _ |- _ => apply genFresh_spec in H
+    end;
+    try (specializes IHe1; [ eassumption | ]);
+    try (specializes IHe2; [ eassumption | ]);
+    try (specializes IHe3; [ eassumption | ]);
+    set_solver var.
+  Qed.
+
+  Lemma compile_modifies_resVar: forall l G t (e: expr l G t) s ngs ngs' resVar,
+    compile ngs e = (s, resVar, ngs') ->
+    resVar \in (modVars s).
+  Proof.
+    intros.
+    destruct e; repeat (inversionss; try destruct_one_match_hyp); simpl in *; set_solver var.
+  Admitted.
+
+  Lemma compile_resVar: forall l G t (e: expr l G t) s ngs ngs' resVar,
+    compile ngs e = (s, resVar, ngs') ->
+    ~ resVar \in (allFreshVars ngs').
+  Proof.
+    intros. destruct e; repeat (inversionss; try destruct_one_match_hyp); simpl in *;
+    repeat match goal with
+    | H: _ |- _ => apply genFresh_spec in H
+    end;
+    set_solver var.
+  Admitted.
+
+  Lemma compile_modVars_spec: forall l G t (e: expr l G t) s ngs ngs' resVar,
+    compile ngs e = (s, resVar, ngs') ->
+    subset (modVars s) (diff (allFreshVars ngs) (allFreshVars ngs')).
+  Proof.
+  Admitted. (*
+    induction e; intros; repeat (inversionss; try destruct_one_match_hyp);
+    admit_if_TODO;
+    simpl;
+    try (specializes IHe1; [ eassumption | ]);
+    try (specializes IHe2; [ eassumption | ]);
+    try (specializes IHe3; [ eassumption | ]);
+    repeat match goal with
+    | H: _ |- _ => apply genFresh_spec in H
+    | H: _ |- _ => apply compile_freshVarUsage in H
+    end;
+    set_solver var.
+  *)
+
+
+  Ltac pose_flatten_var_ineqs :=
+    repeat match goal with
+    | H: _ |- _ => unique apply compile_freshVarUsage in copy of H
+    | H: _ |- _ => unique apply modVarsSound in copy of H
+    | H: _ |- _ => unique apply compile_modifies_resVar in copy of H
+    | H: _ |- _ => unique apply compile_modVars_spec in copy of H
+    end.
+
+  Tactic Notation "nofail" tactic3(t) := first [ t | fail 1000 "should not have failed"].
+
+  Ltac fuel_increasing_rewrite :=
+    match goal with
+    | Ev: eval_stmt ?Fuel1 ?initial ?s = ?final
+      |- context [eval_stmt ?Fuel2 ?initial ?s]
+      => let IE := fresh in assert (Fuel1 <= Fuel2) as IE by omega;
+         apply (increase_fuel_still_Success _ _ _ _ _ IE) in Ev;
+         clear IE;
+         rewrite Ev
+    end.
+
+(*
+  (* Note: If you want to get in the conclusion
+     "only_differ initialL (vars_range firstFree (S resVar)) finalL"
+     this needn't be part of this lemma, because it follows from
+     compile_modVars_spec and modVarsSound *)
+  Lemma compile_correct_aux: forall e ngs1 ngs2 resVar s initialH initialL res,
+    compile ngs1 e = (s, resVar, ngs2) ->
+    extends initialL initialH ->
+    undef initialH (allFreshVars ngs1) ->
+    eval_expr initialH e = Some res ->
+    exists fuel finalL,
+      eval_stmt fuel initialL s = Success finalL /\
+      get finalL resVar = Some res.
+  Proof.
+    induction e; introv F Ex U Ev.
+    - repeat (inversionss; try destruct_one_match_hyp).
+      exists 1%nat (put initialL resVar res).
+      split; state_calc.
+    - repeat (inversionss; try destruct_one_match_hyp).
+      exists 1%nat (put initialL resVar res). repeat split.
+      + simpl. unfold extends in Ex. apply Ex in H0. rewrite H0. simpl. reflexivity.
+      + state_calc.
+    - repeat (inversionss; try destruct_one_match_hyp).
+      pose_flatten_var_ineqs.
+      specialize (IHe1 _ _ _ _ _ _ w0 E Ex).
+      specializes IHe1. {
+        clear IHe2.
+        state_calc.
+      }
+      { assumption. }
+      destruct IHe1 as [fuel1 [midL [Ev1 G1]]].
+      progress pose_flatten_var_ineqs.
+      specialize (IHe2 _ _ _ _ initialH midL w1 E0).
+      specializes IHe2.
+      { state_calc. }
+      { state_calc. }
+      { assumption. }
+      destruct IHe2 as [fuel2 [preFinalL [Ev2 G2]]].
+      remember (Datatypes.S (Datatypes.S (fuel1 + fuel2))) as f0.
+      remember (Datatypes.S (fuel1 + fuel2)) as f.
+      exists (Datatypes.S f0) (put preFinalL resVar (Op.eval_binop op w0 w1)).
+      pose_flatten_var_ineqs.
+      split; [|apply get_put_same].
+      simpl. fuel_increasing_rewrite.
+      subst f0. simpl. fuel_increasing_rewrite.
+      subst f. simpl.
+      assert (get preFinalL v = Some w0) as G1'. {
+        state_calc.
+      }
+      rewrite G1'. simpl. rewrite G2. simpl. reflexivity.
+  Qed.
+
+  Lemma flattenStmt_correct_aux:
+    forall fuelH sH sL ngs ngs' initialH finalH initialL,
+    flattenStmt ngs sH = (sL, ngs') ->
+    extends initialL initialH ->
+    undef initialH (allFreshVars ngs) ->
+    disjoint (modVars sH) (allFreshVars ngs) ->
+    eval_stmt fuelH initialH sH = Some finalH ->
+    exists fuelL finalL,
+      eval_stmt fuelL initialL sL = Success finalL /\
+      extends finalL finalH.
+  Proof.
+    induction fuelH; introv F Ex U Di Ev; [solve [inversionss] |].
+    destruct sH.
+    - apply invert_eval_SSet in Ev.
+      destruct Ev as [v [Ev Eq]].
+      repeat (inversionss; try destruct_one_match_hyp).
+      pose proof (compile_correct_aux _ _ _ _ _ _ _ _ E Ex U Ev) as P.
+      destruct P as [fuelL [prefinalL [Evs G]]].
+      remember (Datatypes.S fuelL) as SfuelL.
+      exists (Datatypes.S SfuelL). eexists. repeat split.
+      + simpl.
+        assert (eval_stmt SfuelL initialL s = Success prefinalL) as Evs'. {
+          eapply increase_fuel_still_Success; [|eassumption]. omega.
+        }
+        rewrite Evs'. subst SfuelL. simpl. rewrite G. simpl. reflexivity.
+      + clear IHfuelH.
+        pose_flatten_var_ineqs.
+        state_calc.
+    - inversions F. repeat destruct_one_match_hyp. destruct_pair_eqs. subst.
+      apply invert_eval_SIf in Ev.
+      destruct Ev as [cv [Evc Ev]].
+      pose_flatten_var_ineqs.
+      rename cond into condH, s into condL, s0 into sL1, s1 into sL2.
+      pose proof (compile_correct_aux _ _ _ _ _ _ _ cv E Ex) as P.
+      specializes P; [eassumption|eassumption|].
+      destruct P as [fuelLcond [initial2L [Evcond G]]].
+      destruct Ev as [[Ne EvThen] | [Eq EvElse]]; pose_flatten_var_ineqs.
+      + specialize (IHfuelH sH1 sL1 n n0 initialH finalH initial2L E0).
+        specializes IHfuelH.
+        * state_calc.
+        * state_calc.
+        * simpl in Di.
+          set_solver var.
+        * exact EvThen.
+        * destruct IHfuelH as [fuelL [finalL [Evbranch Ex2]]].
+          exists (S (S (fuelLcond + fuelL))). eexists.
+          refine (conj _ Ex2).
+          remember (S (fuelLcond + fuelL)) as tempFuel.
+          simpl.
+          fuel_increasing_rewrite.
+          subst tempFuel.
+          simpl. rewrite G. simpl. destruct_one_match; [contradiction|].
+          fuel_increasing_rewrite.
+          reflexivity.
+      + specialize (IHfuelH sH2 sL2 _ _ initialH finalH initial2L E1).
+        specializes IHfuelH.
+        * state_calc.
+        * state_calc.
+        * simpl in Di.
+          set_solver var.
+        * exact EvElse.
+        * destruct IHfuelH as [fuelL [finalL [Evbranch Ex2]]].
+          exists (S (S (fuelLcond + fuelL))). eexists.
+          refine (conj _ Ex2).
+          remember (S (fuelLcond + fuelL)) as tempFuel.
+          simpl.
+          fuel_increasing_rewrite.
+          subst tempFuel.
+          simpl. rewrite G. simpl. destruct_one_match; [|contradiction].
+          fuel_increasing_rewrite.
+          reflexivity.
+    - apply invert_eval_SWhile in Ev.
+      simpl in Di.
+      pose proof F as F0.
+      simpl in F. do 3 destruct_one_match_hyp. destruct_pair_eqs. subst.
+      rename s into sCond, s0 into sBody.
+      destruct Ev as [cv [EvcondH Ev]].
+      pose proof (compile_correct_aux _ _ _ _ _ _ _ cv E Ex) as P.
+      specializes P; [eassumption|eassumption|].
+      destruct P as [fuelLcond [initial2L [EvcondL G]]].
+      destruct Ev as [Ev | Ev]; pose_flatten_var_ineqs.
+      + destruct Ev as [Ne [middleH [Ev1H Ev2H]]].
+        specialize IHfuelH with (1 := E0) (5 := Ev1H) as IH.
+        specialize (IH initial2L).
+        specializes IH.
+        { state_calc. }
+        { state_calc. }
+        { set_solver var. }
+        destruct IH as [fuelL1 [middleL [EvL1 Ex1]]].
+        pose_flatten_var_ineqs.
+        specialize IHfuelH with (initialL := middleL) (1 := F0) (5 := Ev2H).
+        specializes IHfuelH.
+        { state_calc. }
+        { pose proof (modVarsSound _ _ _ _ Ev1H) as D1.
+          state_calc. }
+        { set_solver var. }
+        destruct IHfuelH as [fuelL2 [finalL [EvL2 Ex2]]].
+        exists (S (fuelL1 + fuelL2 + fuelLcond)) finalL.
+        refine (conj _ Ex2).
+        simpl.
+        fuel_increasing_rewrite.
+        rewrite G. simpl. destruct_one_match; [contradiction|].
+        fuel_increasing_rewrite.
+        fuel_increasing_rewrite.
+        reflexivity.
+      + destruct Ev as [? ?]. subst.
+        exists (S fuelLcond) initial2L.
+        split; [|state_calc].
+        simpl.
+        fuel_increasing_rewrite.
+        rewrite G. simpl. destruct_one_match; [|contradiction]. reflexivity.
+    - apply invert_eval_SSeq in Ev.
+      destruct Ev as [middleH [Ev1 Ev2]].
+      simpl in F. do 2 destruct_one_match_hyp. inversions F.
+      pose proof IHfuelH as IHfuelH2.
+      specializes IHfuelH.
+      1: exact E. 1: exact Ex. 3: exact Ev1.
+      { clear IHfuelH2. state_calc. }
+      { simpl in Di. set_solver var. }
+      destruct IHfuelH as [fuelL1 [middleL [EvL1 Ex1]]].
+      rename IHfuelH2 into IHfuelH.
+      rename s into sL1, s0 into sL2.
+      pose_flatten_var_ineqs.
+      simpl in Di.
+      pose proof (modVarsSound _ _ _ _ Ev1) as D1.
+      specialize (IHfuelH sH2 sL2 _ _ middleH finalH middleL E0).
+      specializes IHfuelH.
+      1: exact Ex1. 3: exact Ev2.
+      { state_calc. }
+      { state_calc. }
+      destruct IHfuelH as [fuelL2 [finalL [EvL2 Ex2]]].
+      exists (S (fuelL1 + fuelL2)) finalL.
+      refine (conj _ Ex2).
+      simpl.
+      fuel_increasing_rewrite. fuel_increasing_rewrite. reflexivity.
+    - apply invert_eval_SSkip in Ev. subst finalH.
+      simpl in F. inversions F.
+      exists 1%nat initialL. auto.
+  Qed.
+*)
+End LLG2FlatImp.
